WIP: synchronise the topmost stk of the call-stack with the current stack

theories/examples/switcher/switcher_preamble.v
@@ -31,18 +31,14 @@ Section Switcher_preamble.
   Definition export_table_entryN (C : CmptName) (a : Addr) : namespace :=
     (export_tableN C) .@ "entry" .@ a.
 
-  Program Definition execute_entry_point_register (wpcc wcgp : Word) :
+  Program Definition execute_entry_point_register (wpcc wcgp wstk : Word) :
     (WORLD -n> (leibnizO CmptName) -n> (leibnizO Reg) -n> iPropO Σ) :=
     λne (W : WORLD) (C : CmptName) (reg : leibnizO Reg),
       (full_map reg ∧
        ⌜ reg !! PC = Some wpcc ⌝ ∧
        ⌜ reg !! cgp = Some wcgp ⌝ ∧
        ⌜ reg !! cra = Some (WSentry XSRW_ Local b_switcher e_switcher a_switcher_return) ⌝ ∧
-       (∀ (wstk : Word),
-          (⌜reg !! csp = Some wstk⌝ →
-           (⌜ ∃ csp_b csp_e, wstk = (WCap RWL Local csp_b csp_e csp_b) ⌝ ∧ interp W C wstk))
-       )
-       ∧
+       ⌜ reg !! csp = Some wstk ⌝ ∗ interp W C wstk ∗
        (∀ (r : RegName) (v : Word), (⌜r ∉ ({[PC; cra; cgp; csp]} : gset RegName)⌝ → ⌜reg !! r = Some v⌝ → interp W C v))
       (* NOTE I think the zeroes are not necessary and we never rely in it *)
        (* ∧ *)
@@ -51,16 +47,35 @@ Section Switcher_preamble.
       )%I.
   Solve All Obligations with solve_proper.
 
+  (* TODO move in machine_base *)
+  Definition get_b (w : Word) :=
+    match w with
+    | WCap _ _ b _ _ => Some b
+    | _ => None
+    end.
+
+  Definition csp_sync cstk a_stk e_stk :=
+    match cstk with
+    | frm::_ =>
+        get_a frm.(wstk) = Some a_stk
+        ∧ get_e frm.(wstk) = Some e_stk
+    | _ => True
+    end
+  .
+
   Program Definition execute_entry_point
     (wpcc wcgp : Word) (regs : Reg) (cstk : CSTK) (Ws : list WORLD) (Cs : list CmptName)
     : (WORLD -n> (leibnizO CmptName) -n> iPropO Σ) :=
     (λne (W : WORLD) (C : CmptName),
-      ( interp_continuation cstk Ws Cs
+      ∀ a_stk e_stk,
+       let a_stk4 := (a_stk ^+4)%a in
+       ( interp_continuation cstk Ws Cs
          ∗ ⌜frame_match Ws Cs cstk W C⌝
-         ∗ (execute_entry_point_register wpcc wcgp W C regs)
+         ∗ (execute_entry_point_register wpcc wcgp (WCap RWL Local a_stk4 e_stk a_stk4) W C regs)
          ∗ registers_pointsto regs
          ∗ region W C
          ∗ sts_full_world W C
+         ∗ ⌜csp_sync cstk a_stk e_stk⌝
          ∗ cstack_frag cstk
          ∗ na_own logrel_nais ⊤
            -∗ interp_conf W C)
