theories/examples/counter/counter_spec.v
@@ -33,7 +33,7 @@ Section Counter.
 
     (C_f : Sealable)
 
-    (W_init_C : WORLD)
+    (W0 : WORLD)
 
     (Ws : list WORLD)
     (Cs : list CmptName)
@@ -55,7 +55,9 @@ Section Counter.
     (cgp_b + length counter_main_data)%a = Some cgp_e ->
     (pc_b + length imports)%a = Some pc_a ->
 
-    frame_match Ws Cs cstk W_init_C C ->
+    frame_match Ws Cs cstk W0 C ->
+    csp_sync cstk (csp_b ^+ -4)%a csp_e ->
+
     (
       na_inv logrel_nais Nswitcher switcher_inv
       (* initial memory layout *)
@@ -75,29 +77,30 @@ Section Counter.
       ∗ cra ↦ᵣ WSentry XSRW_ Local b_switcher e_switcher a_switcher_return
       ∗ ( [∗ map] r↦w ∈ rmap, r ↦ᵣ w )
 
-      ∗ region W_init_C C ∗ sts_full_world W_init_C C
+      ∗ region W0 C ∗ sts_full_world W0 C
 
       ∗ interp_continuation cstk Ws Cs
 
       ∗ cstack_frag cstk
 
-      ∗ interp W_init_C C (WSealed ot_switcher C_f)
+      ∗ interp W0 C (WSealed ot_switcher C_f)
       ∗ (WSealed ot_switcher C_f) ↦□ₑ 0
-      ∗ interp W_init_C C (WCap RWL Local csp_b csp_e csp_b)
+      ∗ interp W0 C (WCap RWL Local csp_b csp_e csp_b)
 
       ⊢ WP Seq (Instr Executable) {{ v, ⌜v = HaltedV⌝ → na_own logrel_nais ⊤ }})%I.
   Proof.
     intros imports; subst imports.
     iIntros (HNswitcher_counter Hrmap_dom Hrmap_init HsubBounds
-               Hcgp_contiguous Himports_contiguous Hframe_match
+               Hcgp_contiguous Himports_contiguous Hframe_match Hcsp_sync
             )
+         ∗ ⌜csp_sync cstk a_stk e_stk⌝
       "(#Hswitcher & #Hmem & Hna
       & HPC & Hcgp & Hcsp & Hcra & Hrmap
-      & HWreg_C & HWstd_full_C
+      & Hr_C & Hsts_C
       & HK
       & Hcstk_frag
-      & #Hinterp_C_f & #Hentry_C_f
-      & #Hinterp_Winit_C_csp
+      & #Hinterp_W0_C_f & #Hentry_C_f
+      & #Hinterp_W0_csp
       )".
     iMod (na_inv_acc with "Hmem Hna")
       as "(( %cnt & >Himports_main & >Hcode_main & >Hcgp_main & >%Hcnt) & Hna & Hmem_close)"; auto.
@@ -130,45 +133,19 @@ Section Counter.
     { transitivity (Some (pc_b ^+ 2)%a); auto; solve_addr. }
     { solve_addr. }
 
+
     (* Revoke the world to get the stack frame *)
     set (stk_frame_addrs := finz.seq_between csp_b csp_e).
-    iAssert ([∗ list] a ∈ stk_frame_addrs, ⌜W_init_C.1 !! a = Some Temporary⌝)%I as "Hstack_temporary".
-    { iApply (writeLocalAllowed_valid_cap_implies_full_cap with "Hinterp_Winit_C_csp"); eauto. }
+    iAssert ([∗ list] a ∈ stk_frame_addrs, ⌜W0.1 !! a = Some Temporary⌝)%I as "Hstk_frm_tmp_W0".
+    { iApply (writeLocalAllowed_valid_cap_implies_full_cap with "Hinterp_W0_csp"); eauto. }
 
-    iMod (monotone_revoke_stack with "[$Hinterp_Winit_C_csp $HWstd_full_C $HWreg_C]")
-        as (l_unk) "(%Hl_unk & HWstd_full_C & HWreg_C & Hstk & Hrevoked_rest)".
-    iAssert (
-        |={⊤}=>
-          ▷ ([∗ list] a ∈ finz.seq_between csp_b csp_e,
-             closing_revoked_resources W_init_C C a
-             ∗ ⌜(revoke W_init_C).1 !! a = Some Revoked⌝
-             ∗ ∃ v, a ↦ₐ v
-          )
-      )%I with "[Hstk]" as ">Hstk".
-    {
-      rewrite !big_sepL_sep.
-      iDestruct "Hstk" as "[Hstk $]".
-      iDestruct (big_sepL_later_2 with "Hstk") as "Hstk".
-      iIntros "!>!>".
-      rewrite -big_sepL_sep.
-      iApply (big_sepL_impl with "Hstk").
-      iModIntro; iIntros (k a Hx) "Hrev".
-      iDestruct (close_revoked_resources with "Hrev") as (v) "[$ $]".
-    }
-    iAssert (
-        ▷
-        (∃ stk_mem,
-         ([∗ list] a ∈ finz.seq_between csp_b csp_e,
-          closing_revoked_resources W_init_C C a ∗ ⌜(revoke W_init_C).1 !! a = Some Revoked⌝)
-         ∗ [[ csp_b , csp_e ]] ↦ₐ [[ stk_mem ]])
-      )%I with "[Hstk]" as (stk_mem) "[Hclose_res >Hcsp_stk]".
-    { iNext.
-      rewrite !big_sepL_sep.
-      iDestruct "Hstk" as "(Hclose & Hrev & Hv)".
-      iDestruct (big_sepL_sep with "[$Hclose $Hrev]") as "$".
-      by iApply region_addrs_exists.
-    }
-    set (W1 := revoke W_init_C).
+    iMod (monotone_revoke_stack_alt with "[$Hinterp_W0_csp $Hsts_C $Hr_C]")
+        as (l) "(%Hl_unk & Hsts_C & Hr_C & #Hfrm_close_W0 & >[%stk_mem Hstk] & Hrevoked_l)".
+    (* iDestruct (big_sepL2_disjoint_pointsto with "[$Hstk $Hcgp_b]") as "%Hcgp_b_stk". *)
+
+    set (W1 := revoke W0).
+    assert (related_sts_priv_world W0 W1) as Hrelared_priv_W0_W1 by eapply revoke_related_sts_priv_world.
+
 
     (* --------------------------------------------------- *)
     (* ----------------- Start the proof ----------------- *)
@@ -225,9 +202,11 @@ Section Counter.
     iInstr "Hcode".
 
     (* Jalr cra ct0; *)
-    iInstr "Hcode" with "Hlc".
+    iInstr "Hcode".
 
     subst hcont; unfocus_block "Hcode" "Hcont" as "Hcode_main".
+
+    (* Close the memory invariant before using the switcher's spec*)
 
     iMod ("Hmem_close" with "[$Hna Himport_switcher Himport_C_f Himports_main $Hcode_main Hcgp_b Hcgp_main]") as "Hna".
     { iExists (cnt+1)%Z.
@@ -272,9 +251,7 @@ Section Counter.
 
     set (rmap' := (delete ca5 _)).
 
-    assert (related_sts_priv_world W_init_C W1) as HWinit_privC_W1.
-    { subst W1; eapply revoke_related_sts_priv_world. }
-
+    (* Show that the arguments are safe, when necessary *)
     iAssert ([∗ map] rarg↦warg ∈ rmap_arg, rarg ↦ᵣ warg
                                            ∗ (if decide (rarg ∈ dom_arg_rmap 0)
                                              then interp W1 C warg
@@ -282,56 +259,96 @@ Section Counter.
             )%I
       with "[Hca0 Hca1 Hca2 Hca3 Hca4 Hca5 Hct0]" as "Hrmap_arg".
     { subst rmap_arg.
-      iAssert (interp W1 C (WInt 0)) as "Hinterp_0".
-      { iEval (rewrite fixpoint_interp1_eq); done. }
-      repeat (iApply big_sepM_insert; [done|iFrame "∗#"]); done.
+      iAssert (interp W1 C (WInt 0)) as "Hinterp_0"; first iApply interp_int.
+      repeat (iApply big_sepM_insert; [done|iFrame "∗#"]).
+      done.
     }
 
+    (* Show that the entry point to C_f is still safe in W1 *)
     iAssert (interp W1 C (WSealed ot_switcher C_f)) as "#Hinterp_W1_C_f".
     { iApply monotone.interp_monotone_sd; eauto. }
+    iClear "Hinterp_W0_C_f".
 
-    iApply (switcher_cc_specification _ W1 _ _ _ _ _ _ _ _ _ _ rmap_arg with
+    (* Prepare the closing resources for the switcher call spec *)
+    iAssert (
+        ([∗ list] a ∈ finz.seq_between csp_b csp_e, closing_revoked_resources W1 C a ∗
+                                                    ⌜W1.1 !! a = Some Revoked⌝)
+      )%I with "[Hfrm_close_W0]" as "Hfrm_close_W1".
+    {
+      iApply (big_sepL_impl with "Hfrm_close_W0").
+      iModIntro; iIntros (k a Ha) "[Hclose %Hrev]".
+      iDestruct (mono_priv_closing_revoked_resources with "Hclose") as "$"; auto.
+    }
+
+    iApply (switcher_cc_specification _ _ _ _ _ _ _ _ _ _ _ _ rmap_arg with
              "[- $Hswitcher $Hna
               $HPC $Hcgp $Hcra $Hcsp $Hct1 $Hcs0 $Hcs1 $Hrmap
-              $Hcsp_stk $HWreg_C $HWstd_full_C $Hcstk_frag
-              $Hinterp_W1_C_f $Hentry_C_f $HK]"); eauto.
+              $Hstk $Hr_C $Hsts_C $Hfrm_close_W1 $Hcstk_frag
+              $Hinterp_W1_C_f $Hentry_C_f $HK]"); eauto; last iFrame.
     { subst rmap'.
       repeat (rewrite dom_delete_L); repeat (rewrite dom_insert_L).
       rewrite /dom_arg_rmap Hrmap_dom.
       set_solver+.
     }
     { by rewrite /is_arg_rmap . }
-    iSplitL "Hrmap_arg"; first done.
-    iSplitL "Hclose_res".
-    { rewrite !big_sepL_sep.
-      iDestruct "Hclose_res" as "[Hclose Hrev]".
-      iSplitL "Hclose".
-      - iApply (big_sepL_impl with "Hclose").
-        iModIntro; iIntros (k a Ha) "Hclose".
-        rewrite /closing_revoked_resources.
-        iDestruct "Hclose" as (???) "(?&?&#Hmono&#Hzcond&#Hrcond&#Hwcond&?)".
-        iExists φ,p,Hpers; iFrame "∗#".
-        iApply "Hzcond"; done.
-      - iApply (big_sepL_impl with "Hrev").
-        iModIntro; iIntros (k a Ha) "Hrev".
-        iDestruct (big_sepL_pure_1 with "Hstack_temporary") as "%Hstack_temporary".
-        subst W1.
-        iPureIntro.
-        apply revoke_lookup_Monotemp.
-        eapply Hstack_temporary; eauto.
-    }
 
     iNext. subst rmap'.
     iIntros (W2 rmap')
-      "(%HW1_pubB_W2 & %Hdom_rmap'
-      & Hna & #Hinterp_cdp & %Hcsp_bounds
-      & HWstd_full_B & HWreg_B & Hclose_reg_B & Hclose_reg_B'
-      & Hcstk_frag & Hrel_stk_B
+      "(%Hrelated_pub_1ext_W2 & %Hdom_rmap
+      & Hna & #Hinterp_W2_csp & %Hcsp_bounds
+      & Hsts_C & Hr_C & Hfrm_close_1 & Hfrm_close_W2
+      & Hcstk_frag & Hrel_stk_C
       & HPC & Hcgp & Hcra & Hcs0 & Hcs1 & Hcsp
       & [%warg0 [Hca0 _] ] & [%warg1 [Hca1 _] ]
-      & Hrmap & Hcsp_stk & HK)".
+      & Hrmap & Hstk & HK)".
     iEval (cbn) in "HPC".
 
+    (* TODO see whether I can make this a lemma *)
+    iEval (rewrite <- (app_nil_r (finz.seq_between (csp_b ^+ 4)%a csp_e))) in "Hr_C".
+    rewrite (region_addrs_zeroes_split _ (csp_b ^+4)%a).
+    2: { split; solve_addr+Hcsp_bounds. }
+    set (lv := region_addrs_zeroes (csp_b ^+4)%a csp_e).
+    iDestruct (region_pointsto_split _ _ (csp_b ^+4)%a with "Hstk") as "[Hstk' Hstk]".
+    { split; solve_addr+Hcsp_bounds. }
+    { by rewrite length_replicate. }
+    iAssert (
+       [∗ list] a ; v ∈ finz.seq_between (csp_b ^+ 4)%a csp_e ; lv, a ↦ₐ v ∗ closing_resources interp W2 C a v
+      )%I with "[Hfrm_close_W2 Hstk]" as "Hfrm_close_W2".
+    { rewrite /region_pointsto.
+      iDestruct (big_sepL2_sep_sepL_l  with "[$Hfrm_close_W2 $Hstk]") as "H".
+      iApply (big_sepL2_impl with "H").
+      iIntros "!> % % % % % [? $]"; iFrame.
+      subst lv; apply lookup_replicate in H0 as [-> _]; done.
+    }
+    iDestruct (
+        ftlr_switcher_return.region_close_list_interp_gen
+          with "[$Hr_C $Hfrm_close_W2]"
+      ) as "Hr_C".
+    { apply finz_seq_between_NoDup. }
+    { set_solver+. }
+    { subst lv; by rewrite length_replicate finz_seq_between_length. }
+    rewrite -region_open_nil.
+
+    assert (related_sts_pub_world W1 W2) as Hrelated_pub_W1_W2.
+    {
+      eapply related_sts_pub_trans_world ; eauto.
+      apply related_sts_pub_update_multiple_temp.
+      apply Forall_forall; intros a Ha.
+      eapply revoke_lookup_Monotemp.
+      destruct Hl_unk as [_ Htemp]; apply Htemp.
+      apply elem_of_app; right.
+      rewrite !elem_of_finz_seq_between in Ha |- *; solve_addr+Ha.
+    }
+
+    (* Revoke the world again to get the points-to of the stack *)
+    clear stk_mem.
+    iMod (monotone_revoke_stack_alt with "[$Hinterp_W2_csp $Hsts_C $Hr_C]")
+        as (l') "(%Hl_unk' & Hsts_C & Hr_C & Hfrm_close_W2 & >[%stk_mem Hstk] & Hrevoked_l')".
+    iDestruct (region_pointsto_split with "[$Hstk' $Hstk]") as "Hstk"; auto.
+    { by rewrite length_replicate. }
+    set (W3 := revoke W2).
+
+    (* simplify the knowledge about the new rmap *)
     iDestruct (big_sepM_sep with "Hrmap") as "[Hrmap Hrmap_zero]".
     iDestruct (big_sepM_pure with "Hrmap_zero") as "%Hrmap_zero".
     assert (∀ r : RegName, r ∈ dom rmap' → rmap' !! r = Some (WInt 0)) as Hrmap_init'.
@@ -342,6 +359,10 @@ Section Counter.
       by cbn in Hr' ; simplify_eq.
     }
     iClear "Hrmap_zero".
+
+    (* --------------------------------------------------- *)
+    (* ----------------- BLOCK 4: RETURN ----------------- *)
+    (* --------------------------------------------------- *)
 
     iMod (na_inv_acc with "Hmem Hna")
       as "(( %cnt & >Himports_main & >Hcode_main & >Hcgp_main & >%Hcnt) & Hna & Hmem_close)"; auto.
@@ -358,15 +379,18 @@ Section Counter.
 
     (* Put all the registers under the same map *)
     iDestruct (big_sepM_insert _ _ cs0 with "[$Hrmap $Hcs0]") as "Hrmap".
-    { repeat (rewrite lookup_insert_ne; auto); apply not_elem_of_dom_1; rewrite Hdom_rmap'; set_solver+. }
+    { repeat (rewrite lookup_insert_ne; auto); apply not_elem_of_dom_1; rewrite Hdom_rmap; set_solver+. }
     iDestruct (big_sepM_insert _ _ cs1 with "[$Hrmap $Hcs1]") as "Hrmap".
-    { repeat (rewrite lookup_insert_ne; auto); apply not_elem_of_dom_1; rewrite Hdom_rmap'; set_solver+. }
+    { repeat (rewrite lookup_insert_ne; auto); apply not_elem_of_dom_1; rewrite Hdom_rmap; set_solver+. }
     iDestruct (big_sepM_insert _ _ ca0 with "[$Hrmap $Hca0]") as "Hrmap".
-    { repeat (rewrite lookup_insert_ne; auto); apply not_elem_of_dom_1; rewrite Hdom_rmap'; set_solver+. }
+    { repeat (rewrite lookup_insert_ne; auto); apply not_elem_of_dom_1; rewrite Hdom_rmap; set_solver+. }
     iDestruct (big_sepM_insert _ _ ca1 with "[$Hrmap $Hca1]") as "Hrmap".
-    { repeat (rewrite lookup_insert_ne; auto); apply not_elem_of_dom_1; rewrite Hdom_rmap'; set_solver+. }
+    { repeat (rewrite lookup_insert_ne; auto); apply not_elem_of_dom_1; rewrite Hdom_rmap; set_solver+. }
 
-    (* TODO Apply the switcher's return specification *)
+    clear dependent wcs0 wcs1 wct0 wct1 a_fetch1 a_fetch2 a_callB a_ret.
+    iClear "Hmem Hentry_C_f".
+    subst W3.
+    (* (* TODO Apply the switcher's return specification *) *)
 
   Admitted.
 
@@ -378,7 +402,7 @@ Section Counter.
 
     (C_f : Sealable)
 
-    (W_init_C : WORLD)
+    (W0 : WORLD)
 
     (Ws : list WORLD)
     (Cs : list CmptName)
@@ -406,27 +430,25 @@ Section Counter.
             ∗ [[ cgp_b, cgp_e ]] ↦ₐ [[ [WInt cnt] ]]
             ∗ ⌜ (0 <= cnt)%Z ⌝
         )
-    ∗ interp W_init_C C (WSealed ot_switcher C_f)
+    ∗ interp W0 C (WSealed ot_switcher C_f)
     ∗ (WSealed ot_switcher C_f) ↦□ₑ 0
     ⊢ execute_entry_point
       (WCap RX Global pc_b pc_e pc_a) (WCap RW Global cgp_b cgp_e cgp_b) rmap
-      cstk Ws Cs W_init_C C.
+      cstk Ws Cs W0 C.
   Proof.
     intros imports; subst imports.
     iIntros (HNswitcher_counter HsubBounds
                Hcgp_contiguous Himports_contiguous)
       "(#Hswitcher & #Hmain & #Hinterp_C_f & #HentryC_f)
-      (HK & %Hframe_match & Hregister_state & Hrmap & HWreg_C & HWstd_full_C & Hcstk & Hna)".
-    iDestruct "Hregister_state" as "(%Hfullrmap & %HPC & %Hcgp & %Hcra & Hcsp & Hinterp_rmap)".
+      % % (HK & %Hframe_match & Hregister_state & Hrmap & Hr_C & Hsts_C & %Hsync_csp & Hcstk & Hna)".
+    iDestruct "Hregister_state" as "(%Hfullrmap & %HPC & %Hcgp & %Hcra & %Hcsp & #Hinterp_csp & Hinterp_rmap)".
     rewrite /interp_conf.
     rewrite /registers_pointsto.
 
     iDestruct (big_sepM_delete _ _ PC with "Hrmap") as "[HPC Hrmap]"; first by simplify_map_eq.
     iDestruct (big_sepM_delete _ _ cgp with "Hrmap") as "[Hcgp Hrmap]"; first by simplify_map_eq.
-    pose proof (Hfullrmap csp) as [wcsp Hwcsp].
-    iDestruct ("Hcsp" $! wcsp Hwcsp) as "[H Hinterp_csp]"; iDestruct "H" as (??) "->".
-    iDestruct (big_sepM_delete _ _ cra with "Hrmap") as "[Hcra Hrmap]"; first by simplify_map_eq.
     iDestruct (big_sepM_delete _ _ csp with "Hrmap") as "[Hcsp Hrmap]"; first by simplify_map_eq.
+    iDestruct (big_sepM_delete _ _ cra with "Hrmap") as "[Hcra Hrmap]"; first by simplify_map_eq.
 
     iApply counter_spec; last iFrame "∗#"; eauto.
     { repeat (rewrite dom_delete_L).
@@ -438,6 +460,8 @@ Section Counter.
       repeat (rewrite lookup_delete_ne; last set_solver).
       set_solver.
     }
-  Qed.
+    replace (((a_stk ^+ 4) ^+ -4)%a)%a with a_stk; first done.
+    admit.
+  Admitted.
 
 End Counter.
