theories/examples/switcher/switcher_spec_return.v
@@ -31,38 +31,36 @@ Section Switcher.
 
   Lemma switcher_ret_specification
     (Nswitcher : namespace)
-    (W0 W : WORLD)
+    (W0 Wcur : WORLD)
     (C : CmptName)
     (rmap : Reg)
-    (csp_e csp_b cgp_b cgp_e: Addr)
-    (l_unk : list Addr)
+    (csp_e csp_b cgp_e: Addr)
+    (l : list Addr)
     (stk_mem : list Word)
     (cstk : CSTK) (Ws : list WORLD) (Cs : list CmptName)
     (wca0 wca1 : Word)
     :
     dom rmap = all_registers_s ∖ ({[ PC ; csp ; ca0 ; ca1 ]} ) ->
     frame_match Ws Cs cstk W0 C ->
-    NoDup (l_unk ++ finz.seq_between csp_b csp_e) ->
-    (∀ a : finz MemNum, (std W0) !! a = Some Temporary ↔ a ∈ l_unk ++ finz.seq_between csp_b csp_e) ->
-
+    csp_sync cstk (csp_b ^+ -4)%a csp_e ->
+    NoDup (l ++ finz.seq_between csp_b csp_e) ->
+    (∀ a : finz MemNum, W0.1 !! a = Some Temporary ↔ a ∈ l ++ finz.seq_between csp_b csp_e) ->
 
     (* Switcher Invariant *)
     na_inv logrel_nais Nswitcher switcher_inv
-    ∗ ([∗ list] a ∈ finz.seq_between (csp_b ^+ 4)%a csp_e, closing_resources interp W C a (WInt 0))
-    ∗ ([∗ list] a ∈ finz.seq_between (csp_b ^+ 4)%a csp_e, ⌜W.1 !! a = Some Temporary⌝)
     ∗ [[csp_b,csp_e]]↦ₐ[[stk_mem]]
     ∗ cstack_frag cstk
     ∗ interp_continuation cstk Ws Cs
-    ∗ sts_full_world W C
+    ∗ sts_full_world (revoke Wcur) C
     ∗ na_own logrel_nais ⊤
     ∗ PC ↦ᵣ WCap XSRW_ Local b_switcher e_switcher a_switcher_return
-    ∗ open_region_many W C (finz.seq_between (csp_b ^+ 4)%a csp_e)
-    ∗ ([∗ list] a ∈ l_unk,
+    ∗ region (revoke Wcur) C
+    ∗ ([∗ list] a ∈ l,
           (∃ (p : Perm) (P : WORLD * CmptName * Word → iPropI Σ),
               ⌜∀ Wv : WORLD * CmptName * Word, Persistent (P Wv)⌝
               ∗ temp_resources W0 C P a p
               ∗ rel C a p P)
-          ∗ ⌜(std W) !! a = Some Revoked⌝)
+          ∗ ⌜(std (revoke W0)) !! a = Some Revoked⌝)
     ∗ ([∗ map] k↦y ∈ rmap, k ↦ᵣ y)
     ∗ ca0 ↦ᵣ wca0
     ∗ ca1 ↦ᵣ wca1
@@ -70,8 +68,8 @@ Section Switcher.
     ⊢ WP Seq (Instr Executable)
       {{ v, ⌜v = HaltedV⌝ → na_own logrel_nais ⊤ }}.
   Proof.
-    iIntros (Hrmap Hframe Hnodup_revoked Htemp_revoked)
-      "(#Hswitcher & Hcls_stk & #Hstktemp & Hstk & Hcstk & Hcont & Hsts & Hna
+    iIntros (Hrmap Hframe Hcsp_sync Hnodup_revoked Htemp_revoked)
+      "(#Hswitcher & Hstk & Hcstk & HK & Hsts & Hna
     & HPC & Hr & Hrevoked & Hrmap & Hca0 & Hca1 & Hcsp)".
 
     (* --- Extract the code from the invariant --- *)
@@ -90,16 +88,30 @@ Section Switcher.
     assert (SubBounds b_switcher e_switcher a_switcher_return (a_switcher_call ^+(length switcher_instrs))%a)
       by solve_addr.
 
-    focus_block_nochangePC 1 "Hcode" as a_ret Ha_ret "Hcode" "Hcls". iHide "Hcls" as hcont.
+    codefrag_facts "Hcode".
+    rewrite /switcher_instrs /switcher_call_instrs /switcher_return_instrs.
+    rewrite -!app_assoc.
+    focus_block_nochangePC 6 "Hcode" as a_ret Ha_ret "Hcode" "Hcont"; iHide "Hcont" as hcont.
     iHide "Hclose_switcher_inv" as hclose_switcher_inv.
     iHide "Hswitcher" as hinv_switcher.
-    replace a_ret with a_switcher_return by solve_addr.
-    codefrag_facts "Hcode".
+    replace a_switcher_return with a_ret by solve_addr.
 
-    assert (is_Some (rmap !! ctp)) as [??];[apply elem_of_dom;rewrite Hrmap;set_solver-|].
-    iExtract "Hrmap" ctp as "Hctp".
+    assert (is_Some (rmap !! cra)) as [??];[apply elem_of_dom;rewrite Hrmap;set_solver-|].
+    iExtract "Hrmap" cra as "Hcra".
     assert (is_Some (rmap !! cgp)) as [??];[apply elem_of_dom;rewrite Hrmap;set_solver-|].
     iExtract "Hrmap" cgp as "Hcgp".
+    assert (is_Some (rmap !! ctp)) as [??];[apply elem_of_dom;rewrite Hrmap;set_solver-|].
+    iExtract "Hrmap" ctp as "Hctp".
+    assert (is_Some (rmap !! ca2)) as [??];[apply elem_of_dom;rewrite Hrmap;set_solver-|].
+    iExtract "Hrmap" ca2 as "Hca2".
+    assert (is_Some (rmap !! cs1)) as [??];[apply elem_of_dom;rewrite Hrmap;set_solver-|].
+    iExtract "Hrmap" cs1 as "Hcs1".
+    assert (is_Some (rmap !! cs0)) as [??];[apply elem_of_dom;rewrite Hrmap;set_solver-|].
+    iExtract "Hrmap" cs0 as "Hcs0".
+    assert (is_Some (rmap !! ct0)) as [??];[apply elem_of_dom;rewrite Hrmap;set_solver-|].
+    iExtract "Hrmap" ct0 as "Hct0".
+    assert (is_Some (rmap !! ct1)) as [??];[apply elem_of_dom;rewrite Hrmap;set_solver-|].
+    iExtract "Hrmap" ct1 as "Hct1".
 
     (* --- ReadSR ctp mtdc --- *)
     iInstr "Hcode"; try solve_pure.
@@ -173,8 +185,10 @@ Section Switcher.
     rename a into a_stk; rename b into b_stk; rename e into e_stk.
     iDestruct "Hcframe_interp" as "(%HWF & -> & Hcframe_interp)".
     destruct HWF as (Hb_a4 & He_a1 & [a_stk4 Ha_stk4]).
+    cbn in Hcsp_sync; destruct Hcsp_sync as [ Ha He ]; simplify_eq.
+    set (a_stk := (csp_b ^+ -4)%a).
 
-    iDestruct "Hcont" as "(Hcont_K & #Hinterp_callee_wstk & Hexec_topmost_frm)".
+    iDestruct "HK" as "(Hcont_K & #Hinterp_callee_wstk & Hexec_topmost_frm)".
 
     rewrite -/(interp_cont).
 
@@ -202,10 +216,11 @@ Section Switcher.
 
     (* --- Lea csp -1 --- *)
     iInstr "Hcode".
-    { by transitivity (Some (a_stk ^+ 3)%a); solve_addr+Ha_stk4. }
+    { transitivity (Some (a_stk ^+ 3)%a); subst a_stk; solve_addr+Ha_stk4. }
 
-    set (stk_len := finz.dist (csp_b ^+ 4)%a csp_e).
+    set (stk_len := finz.dist (a_stk ^+ 4)%a csp_e).
     set (stk_ws := repeat (WInt 0) stk_len).
+    simpl.
 
     (* NOTE in the case of untrusted code calling,
        it means that the addresses (astk, astk+4) are stored in the world,
@@ -223,129 +238,310 @@ Section Switcher.
           ∗ (a_stk ^+ 3)%a ↦ₐ wastk3
           (* ∗ ▷ ([∗ list] a ; v ∈ la ; lv, ▷ closing_resources interp W C a v) *)
           ∗ (⌜if is_untrusted_caller then True else (wastk = wcs0 ∧ wastk1 = wcs1 ∧ wastk2 = wret ∧ wastk3 = wcgp)⌝)
-          ∗ ([∗ list] a ∈ l_unk, (∃ (p : Perm) (P : WORLD * CmptName * Word → iPropI Σ),
-                                      ⌜∀ Wv : WORLD * CmptName * Word, Persistent (P Wv)⌝ ∗
-                                      temp_resources W0 C P a p ∗ rel C a p P) ∗
-               ⌜W.1 !! a = Some Revoked⌝)
+          ∗ ( if is_untrusted_caller
+              then
+                ( ∃ l',
+                    ⌜ l ≡ₚ [a_stk;(a_stk ^+ 1)%a;(a_stk ^+ 2)%a;(a_stk ^+ 3)%a]++l' ⌝
+                    ∗ ([∗ list] a ∈ l', (∃ (p : Perm) (P : WORLD * CmptName * Word → iPropI Σ),
+                                       ⌜∀ Wv : WORLD * CmptName * Word, Persistent (P Wv)⌝ ∗
+                                                                        temp_resources W0 C P a p ∗ rel C a p P) ∗
+                                   ⌜(revoke W0).1 !! a = Some Revoked⌝)
+                    (* ∗ ([∗ list] a ∈ l', (∃ (p' : Perm) (φ : WORLD * CmptName * Word → iPropI Σ), *)
+                    (*                          ⌜∀ Wv : WORLD * CmptName * Word, Persistent (φ Wv)⌝ ∗ ▷ temp_resources W4 C φ a p' ∗ *)
+                    (*                                                           rel C a p' φ) ∗ ⌜(revoke W4).1 !! a = Some Revoked⌝) *)
+                )
+              else
+                ([∗ list] a ∈ l, (∃ (p : Perm) (P : WORLD * CmptName * Word → iPropI Σ),
+                                     ⌜∀ Wv : WORLD * CmptName * Word, Persistent (P Wv)⌝ ∗
+                                                                      temp_resources W0 C P a p ∗ rel C a p P) ∗
+                                 ⌜(revoke W0).1 !! a = Some Revoked⌝
+                )
+            )
       )%I
-      with "[Hcframe_interp Hcls_stk Hrevoked]" as "Hcframe_interp"
+      with "[Hcframe_interp Hrevoked]" as "Hcframe_interp"
     ; [|iDestruct "Hcframe_interp" as
         (wastk wastk1 wastk2 wastk3
         ) "(Ha_stk & Ha_stk1 & Ha_stk2 & Ha_stk3 & %Hwastks & Hrevoked)"
       ].
+    { admit. }
+    (* { *)
+    (*   destruct is_untrusted_caller; cycle 1. *)
+    (*   * iExists wcs0, wcs1, wret, wcgp. *)
+    (*     iDestruct "Hcframe_interp" as "($&$&$&$)". iFrame. *)
+    (*     done. *)
+    (*   * cbn. *)
+    (*     iAssert *)
+    (*       (⌜ ∀ (a : Addr), a ∈ (finz.seq_between b_stk csp_e) → (std W0 !! a) = Some Temporary ⌝)%I *)
+    (*       as "%Hstk_tmp". *)
+    (*     { *)
+    (*       iDestruct (writeLocalAllowed_valid_cap_implies_full_cap with "Hinterp_callee_wstk") as "%Hstk_tmp" ; auto. *)
+    (*       iPureIntro ; intros a Ha. *)
+    (*       apply elem_of_list_lookup_1 in Ha as [k Ha]. *)
+    (*       by eapply Hstk_tmp. *)
+    (*     } *)
+
+    (*     iAssert ( ⌜ a_stk ∈ l ⌝)%I as "%Hastk_unk". *)
+    (*     { *)
+    (*       opose proof (Hstk_tmp a_stk _) as Hastk_tmp. *)
+    (*       { rewrite elem_of_finz_seq_between; subst a_stk; solve_addr+Hb_a4 He_a1 Ha_stk4. } *)
+    (*       apply Htemp_revoked in Hastk_tmp. *)
+    (*       apply elem_of_app in Hastk_tmp as [?|Hcontra]; first done. *)
+    (*       rewrite elem_of_finz_seq_between in Hcontra. *)
+    (*       subst a_stk. *)
+    (*       solve_addr+Hcontra. *)
+    (*     } *)
+    (*     iAssert ( ⌜ (a_stk ^+1)%a ∈ l ⌝)%I as "%Hastk1_unk". *)
+    (*     { *)
+    (*       opose proof (Hstk_tmp (a_stk ^+1)%a _) as Hastk_tmp. *)
+    (*       { rewrite elem_of_finz_seq_between; subst a_stk; solve_addr+Hb_a4 He_a1 Ha_stk4. } *)
+    (*       apply Htemp_revoked in Hastk_tmp. *)
+    (*       apply elem_of_app in Hastk_tmp as [?|Hcontra]; first done. *)
+    (*       rewrite elem_of_finz_seq_between in Hcontra. *)
+    (*       subst a_stk. *)
+    (*       solve_addr+Hcontra. *)
+    (*     } *)
+    (*     iAssert ( ⌜ (a_stk ^+2)%a ∈ l ⌝)%I as "%Hastk2_unk". *)
+    (*     { *)
+    (*       opose proof (Hstk_tmp (a_stk ^+2)%a _) as Hastk_tmp. *)
+    (*       { rewrite elem_of_finz_seq_between; subst a_stk; solve_addr+Hb_a4 He_a1 Ha_stk4. } *)
+    (*       apply Htemp_revoked in Hastk_tmp. *)
+    (*       apply elem_of_app in Hastk_tmp as [?|Hcontra]; first done. *)
+    (*       rewrite elem_of_finz_seq_between in Hcontra. *)
+    (*       subst a_stk. *)
+    (*       solve_addr+Hcontra. *)
+    (*     } *)
+    (*     iAssert ( ⌜ (a_stk ^+3)%a ∈ l ⌝)%I as "%Hastk3_unk". *)
+    (*     { *)
+    (*       opose proof (Hstk_tmp (a_stk ^+3)%a _) as Hastk_tmp. *)
+    (*       { rewrite elem_of_finz_seq_between; subst a_stk; solve_addr+Hb_a4 He_a1 Ha_stk4. } *)
+    (*       apply Htemp_revoked in Hastk_tmp. *)
+    (*       apply elem_of_app in Hastk_tmp as [?|Hcontra]; first done. *)
+    (*       rewrite elem_of_finz_seq_between in Hcontra. *)
+    (*       subst a_stk. *)
+    (*       solve_addr+Hcontra. *)
+    (*     } *)
+    (*     iAssert *)
+    (*       ( ∃ l', *)
+    (*           ⌜ l ≡ₚ [a_stk;(a_stk ^+ 1)%a;(a_stk ^+ 2)%a;(a_stk ^+ 3)%a]++l' ⌝ *)
+    (*           ∗ ([∗ list] a ∈ l', (∃ (p : Perm) (P : WORLD * CmptName * Word → iPropI Σ), *)
+    (*                                   ⌜∀ Wv : WORLD * CmptName * Word, Persistent (P Wv)⌝ ∗ *)
+    (*                                                                    temp_resources W0 C P a p ∗ rel C a p P) ∗ *)
+    (*                               ⌜(revoke W0).1 !! a = Some Revoked⌝) *)
+    (*           ∗ (∃ wastk wastk1 wastk2 wastk3, *)
+    (*                 a_stk ↦ₐ wastk *)
+    (*                 ∗ (a_stk ^+ 1)%a ↦ₐ wastk1 *)
+    (*                 ∗ (a_stk ^+ 2)%a ↦ₐ wastk2 *)
+    (*                 ∗ (a_stk ^+ 3)%a ↦ₐ wastk3 *)
+    (*             ) *)
+    (*       )%I with "[Hrevoked]" *)
+    (*       as (l') "(%Hl_unk'' & Hrevoked_l'' & H)". *)
+    (* { apply NoDup_app in Hnodup_revoked as (Hnodup_revoked & ? & ?). *)
+    (*   apply elem_of_Permutation in Hastk_unk as [l0 Hl0]. *)
+    (*   rewrite Hl0 in Hastk1_unk,Hastk2_unk,Hastk3_unk. *)
+    (*   apply elem_of_cons in Hastk3_unk as [Hcontra | Hastk3_unk]; first (subst a_stk;solve_addr+Hcontra He_a1). *)
+    (*   apply elem_of_cons in Hastk2_unk as [Hcontra | Hastk2_unk]; first (subst a_stk;solve_addr+Hcontra He_a1). *)
+    (*   apply elem_of_cons in Hastk1_unk as [Hcontra | Hastk1_unk]; first (subst a_stk;solve_addr+Hcontra He_a1). *)
+
+    (*   apply elem_of_Permutation in Hastk1_unk as [l1 Hl1]. *)
+    (*   rewrite Hl1 in Hastk2_unk,Hastk3_unk. *)
+    (*   apply elem_of_cons in Hastk3_unk as [Hcontra | Hastk3_unk]; first (subst a_stk;solve_addr+Hcontra He_a1). *)
+    (*   apply elem_of_cons in Hastk2_unk as [Hcontra | Hastk2_unk]; first (subst a_stk;solve_addr+Hcontra He_a1). *)
+
+    (*   apply elem_of_Permutation in Hastk2_unk as [l2 Hl2]. *)
+    (*   rewrite Hl2 in Hastk3_unk. *)
+    (*   apply elem_of_cons in Hastk3_unk as [Hcontra | Hastk3_unk]; first (subst a_stk;solve_addr+Hcontra He_a1). *)
+
+    (*   apply elem_of_Permutation in Hastk3_unk as [l3 Hl3]. *)
+
+    (*   rewrite Hl3 in Hl2; rewrite Hl2 in Hl1; rewrite Hl1 in Hl0. *)
+    (*   clear Hl3 Hl2 Hl1. *)
+
+    (*   iExists l3; iFrame "%". *)
+    (*   iEval (setoid_rewrite Hl0) in "Hrevoked". *)
+    (*   cbn. *)
+    (*   iDestruct "Hrevoked" as "( [Hv0 _] & [Hv1 _] & [Hv2 _] & [Hv3 _] & $)". *)
+    (*   iDestruct "Hv0" as (? ? ?) "[Hv0 _]". *)
+    (*   iDestruct "Hv1" as (? ? ?) "[Hv1 _]". *)
+    (*   iDestruct "Hv2" as (? ? ?) "[Hv2 _]". *)
+    (*   iDestruct "Hv3" as (? ? ?) "[Hv3 _]". *)
+    (*   rewrite /temp_resources. *)
+    (*   iDestruct "Hv0" as (??) "[$ _]". *)
+    (*   iDestruct "Hv1" as (??) "[$ _]". *)
+    (*   iDestruct "Hv2" as (??) "[$ _]". *)
+    (*   iDestruct "Hv3" as (??) "[$ _]". *)
+    (* } *)
+    (* iDestruct "H" as (????) "($&$&$&$)". *)
+    (* by iFrame. *)
+    (* } *)
+
+    (* --- Load cgp csp --- *)
+    iInstr "Hcode".
+    { split ; [ solve_pure | rewrite le_addr_withinBounds ; solve_addr+Ha_stk4 Hb_a4 He_a1 ]. }
+    iEval (cbn) in "Hcgp".
+
+    (* --- Lea csp (-1)%Z --- *)
+    iInstr "Hcode".
+    { by transitivity (Some (a_stk ^+ 2)%a); subst a_stk; solve_addr+Ha_stk4. }
+    replace ((csp_b ^+ -4) ^+ 3)%a with (a_stk ^+ 3)%a by (subst a_stk; solve_addr+Ha_stk4).
+    replace ((csp_b ^+ -4) ^+ 2)%a with (a_stk ^+ 2)%a by (subst a_stk; solve_addr+Ha_stk4).
+
+    (* Load ca2 csp *)
+    iInstr "Hcode".
+    { split ; [ solve_pure | rewrite le_addr_withinBounds ; subst a_stk; solve_addr+Ha_stk4 Hb_a4 He_a1 ]. }
+    iEval (cbn) in "Hca2".
+    (* Lea csp (-1)%Z *)
+    iInstr "Hcode".
+    { by transitivity (Some (a_stk ^+ 1)%a); subst a_stk; solve_addr+Ha_stk4. }
+    (* Load cs1 csp *)
+    iInstr "Hcode".
+    { split ; [ solve_pure | rewrite le_addr_withinBounds ; subst a_stk; solve_addr+Ha_stk4 Hb_a4 He_a1 ]. }
+    iEval (cbn) in "Hcs1".
+    (* Lea csp (-1)%Z *)
+    iInstr "Hcode".
+    { by transitivity (Some a_stk); subst a_stk; solve_addr. }
+    (* Load cs0 csp *)
+    iInstr "Hcode".
+    { split ; [ solve_pure | rewrite le_addr_withinBounds ; subst a_stk; solve_addr+Ha_stk4 Hb_a4 He_a1 ]. }
+    iEval (cbn) in "Hcs0".
+    (* GetE ct0 csp *)
+    iInstr "Hcode".
+    (* GetA ct1 csp *)
+    iInstr "Hcode".
+
+    unfocus_block "Hcode" "Hcont" as "Hcode"; subst hcont.
+
+    (* -------- CLEAR STACK --------- *)
+    focus_block 7 "Hcode" as a7 Ha7 "Hcode" "Hcont"; iHide "Hcont" as hcont.
+    iAssert ([[ a_stk , csp_e ]] ↦ₐ [[wastk :: wastk1 :: wastk2 :: wastk3 :: stk_mem]])%I
+      with "[Ha_stk Ha_stk1 Ha_stk2 Ha_stk3 Hstk]" as "Hstk".
     {
-      destruct is_untrusted_caller; cycle 1.
-      * iExists wcs0, wcs1, wret, wcgp.
-        iDestruct "Hcframe_interp" as "($&$&$&$)". iFrame.
-        cbn.
-        done.
-        (* iSplit;done. *)
-        (* iNext. *)
-        (* iApply (big_sepL2_mono (λ _ a _, closing_resources interp W C a (WInt 0))). *)
-        (* { iIntros (???? ->%elem_of_list_lookup_2%elem_of_list_In%repeat_spec) "HH". *)
-        (*   iFrame. } *)
-        (* iApply big_sepL2_const_sepL_l. iFrame. iPureIntro. *)
-        (* rewrite repeat_length finz_seq_between_length//. *)
-      * cbn.
-        iAssert
-          (⌜ ∀ (a : Addr), a ∈ (finz.seq_between b_stk e_stk) → (std W0 !! a) = Some Temporary ⌝)%I
-          as "%Hstk_tmp".
-        {
-          iDestruct (writeLocalAllowed_valid_cap_implies_full_cap with "Hinterp_callee_wstk") as "%Hstk_tmp" ; auto.
-          iPureIntro ; intros a Ha.
-          apply elem_of_list_lookup_1 in Ha as [k Ha].
-          by eapply Hstk_tmp.
-        }
+      iAssert ([[ (a_stk ^+ 4)%a , csp_e ]] ↦ₐ [[ stk_mem ]])%I with "[Hstk]" as "Hstk".
+      { replace (a_stk ^+ 4)%a with csp_b; first done. subst a_stk;solve_addr+Ha_stk4. }
+      subst a_stk.
+      iDestruct (region_pointsto_cons with "[$Ha_stk3 $Hstk]") as "Hstk"; [solve_addr+Ha_stk4|solve_addr+He_a1|].
+      iDestruct (region_pointsto_cons with "[$Ha_stk2 $Hstk]") as "Hstk"; [solve_addr+Ha_stk4|solve_addr+He_a1|].
+      iDestruct (region_pointsto_cons with "[$Ha_stk1 $Hstk]") as "Hstk"; [solve_addr+Ha_stk4|solve_addr+He_a1|].
+      iDestruct (region_pointsto_cons with "[$Ha_stk $Hstk]") as "Hstk"; [solve_addr+Ha_stk4|solve_addr+He_a1|].
+      iFrame.
+    }
 
-        iAssert ( ⌜ a_stk ∈ l_unk ⌝)%I as "%Hastk_unk".
-        {
-          opose proof (Hstk_tmp a_stk _) as Hastk_tmp.
-          { rewrite elem_of_finz_seq_between; solve_addr+Hb_a4 He_a1 Ha_stk4. }
-          apply Htemp_revoked in Hastk_tmp.
-          apply elem_of_app in Hastk_tmp as [?|Hcontra]; first done.
-          (* TODO it should be that a_stk is (csp_b+4) *)
-          admit.
-        }
+    iApply (clear_stack_spec with "[ - $HPC $Hcsp $Hct0 $Hct1 $Hcode $Hstk]"); eauto; [solve_addr|].
+    iSplitL; cycle 1.
+    { iIntros "!> %"; simplify_eq. }
+    iNext ; iIntros "(HPC & Hcsp & Hct0 & Hct1 & Hcode & Hstk)".
+    unfocus_block "Hcode" "Hcont" as "Hcode"; subst hcont.
+
+    focus_block 8 "Hcode" as a8 Ha8 "Hcode" "Hcont"; iHide "Hcont" as hcont.
+    (* Mov cra ca2 *)
+    iInstr "Hcode" with "Hlc".
+    unfocus_block "Hcode" "Hcont" as "Hcode"; subst hcont.
+
+    (* -------- CLEAR REGISTERS --------- *)
+    focus_block 9 "Hcode" as a9 Ha9 "Hcode" "Hcont"; iHide "Hcont" as hcont.
+    iDestruct (big_sepM_insert_delete with "[$Hrmap $Hct1]") as "Hrmap".
+    rewrite -delete_insert_ne //.
+    iDestruct (big_sepM_insert_delete with "[$Hrmap $Hct0]") as "Hrmap".
+    do 2 (rewrite (delete_commute _ _ ca2); auto).
+    do 2 (rewrite -delete_insert_ne //).
+    iDestruct (big_sepM_insert_delete with "[$Hrmap $Hca2]") as "Hrmap".
+    do 2 (rewrite (delete_commute _ _ ctp); auto).
+    do 3 (rewrite -delete_insert_ne //).
+    iDestruct (big_sepM_insert_delete with "[$Hrmap $Hctp]") as "Hrmap".
+
+    iApply (clear_registers_post_call_spec with "[- $HPC $Hrmap $Hcode]"); try solve_pure.
+    { clear -Hrmap.
+      repeat (rewrite -delete_insert_ne //).
+      repeat (rewrite dom_delete_L).
+      repeat (rewrite dom_insert_L).
+      rewrite Hrmap.
+      set_solver.
+    }
+    iNext; iIntros "H".
+    iDestruct "H" as (arg_rmap') "(%Harg_rmap' & HPC & Hrmap & Hcode)".
+    unfocus_block "Hcode" "Hcont" as "Hcode"; subst hcont.
+
+
+    focus_block 10 "Hcode" as a10 Ha10 "Hcode" "Hcont"; iHide "Hcont" as hcont.
+    (* JmpCap cra *)
+    iInstr "Hcode" with "Hlc".
+    unfocus_block "Hcode" "Hcont" as "Hcode"; subst hcont.
+
+    iHide "Hcode" as hcode.
+    subst a_stk; set (a_stk := (csp_b ^+ -4)%a).
+    (* rewrite (region_addrs_zeroes_split _ (a_stk ^+ 4)%a); last (subst a_stk ; solve_addr+Ha_stk4 Hb_a4 He_a1). *)
+    (* rewrite (region_pointsto_split _ _ (a_stk ^+ 4)%a) *)
+    (* ; [| subst a_stk ; solve_addr+Ha_stk4 Hb_a4 He_a1 | by rewrite /region_addrs_zeroes length_replicate]. *)
+    (* iDestruct "Hstk" as "[Hstk_register_save Hstk]". *)
+
+
+    (* Update the call-stack: depop the topmost frame *)
+    iDestruct (cstack_update _ _ cstk with "[$] [$]") as ">[Hcstk_full Hcstk_frag]".
+
+    (* Close the switcher's invariant *)
+    iDestruct (region_pointsto_cons with "[$Ha_tstk $Htstk]") as "Htstk"; [solve_addr| solve_addr| ].
+    iMod ("Hclose_switcher_inv"
+           with "[Hstk_interp_next $Hna $Hmtdc $Hcode $Hb_switcher Htstk $Hcstk_full $Hp_ot_switcher]")
+      as "Hna".
+    {
+      replace (a_tstk1 ^+ 1)%a with a_tstk by solve_addr.
+      replace (a_tstk ^+ -1)%a with a_tstk1 by solve_addr.
+      iFrame.
+      iNext.
+      iSplit; first (iPureIntro; done).
+      iSplit; first (iPureIntro; solve_addr+Hbounds_tstk_b Hbounds_tstk_e Hlen_cstk Ha_tstk1).
+      iPureIntro; solve_addr+Hbounds_tstk_b  Hlen_cstk Ha_tstk1.
+    }
+
+    (* TODO need to fix the world *)
+
+
+    destruct is_untrusted_caller; cycle 1.
+    - (* Case where caller is trusted, we use the continuation *)
+      destruct Hwastks as (-> & -> & -> & ->).
+      (* TODO need open the world *)
+      (* iEval (rewrite app_nil_r) in "Hr". *)
+      (* iAssert ([[a_stk,e_stk]] ↦ₐ [[region_addrs_zeroes a_stk e_stk%a]])%I with "[Hstk_register_save Hstk]" as "Hstk". *)
+      (* { *)
+      (*   rewrite (region_addrs_zeroes_split a_stk (a_stk ^+4)%a e_stk); last solve_addr+Ha_stk4 He_a1 Hb_a4. *)
+      (*   rewrite region_pointsto_split; first iFrame. *)
+      (*   solve_addr+Ha_stk4 He_a1 Hb_a4. *)
+      (*   by rewrite /region_addrs_zeroes length_replicate. *)
+      (* } *)
+      (* iAssert (([∗ list] a ∈ finz.seq_between (a_stk ^+ 4)%a e_stk, closing_resources interp W C a (WInt 0)))%I *)
+      (*   with "[Hres]" as "Hres". *)
+      (* { iClear "#". *)
+      (*   clear -Hlen_lv. *)
+      (*   iStopProof. *)
+      (*   revert Hlen_lv. *)
+      (*   generalize dependent lv. *)
+      (*   generalize (finz.seq_between (a_stk ^+ 4)%a e_stk) as la. *)
+      (*   induction la; iIntros (lv Hlen) "H"; destruct lv as [|v lv]; simplify_eq; cbn; first done. *)
+      (*   iDestruct "H" as "[Ha H]". *)
+      (*   iDestruct (closing_resources_zeroed with "Ha") as "$". *)
+      (*   by iApply (IHla with "H"). *)
+      (* } *)
+
+      (* here I'm supposed to have fixed the world, so (revoke Wcur) should be fixed *)
+      iAssert (interp (revoke Wcur) C wca0)%I as "#Hinterp_wca0".
+      { admit. (* hypothesis *) }
+      iAssert (interp (revoke Wcur) C wca1)%I as "#Hinterp_wca1".
+      { admit. (* hypothesis *) }
+      iApply ("Hexec_topmost_frm" with
+               "[] [$HPC $Hcra $Hcsp $Hcgp $Hcs0 $Hcs1 $Hca0 $Hca1 $Hinterp_wca0 $Hinterp_wca1
+      $Hrmap $Hstk Hr $Hsts $Hcont_K $Hcstk_frag $Hna]").
+      { admit. (* hypothesis *) }
+      iSplitR.
+      { iPureIntro;rewrite Harg_rmap'; set_solver. }
+      iSplit; first done.
+      iSplit; first done.
+      admit. (* follows from opening the world *)
+
+    - (* Case where caller is untrusted, we use the IH *)
+
+      (* I should know that wastk,... , are interp, because of interp_callee_wstk
+       and fixed world is public *)
+
   Admitted.
-  (*       } *)
-  (*       do 4 (rewrite (finz_seq_between_cons _ (a_stk ^+ 4)%a); last solve_addr+He_a1). *)
-  (*       rewrite (finz_seq_between_empty _ (a_stk ^+ 4)%a); last solve_addr+. *)
-  (*       cbn. *)
-  (*       replace ((a_stk ^+ 1) ^+ 1)%a with (a_stk ^+ 2)%a by solve_addr+Ha_stk4. *)
-  (*       replace ((a_stk ^+ 2) ^+ 1)%a with (a_stk ^+ 3)%a by solve_addr+Ha_stk4. *)
-  (*       cbn. *)
-  (*       iDestruct "Hres" as "(Hres0 & Hres1 & Hres2 & Hres3 & _)". *)
-  (*       iDestruct (opening_closing_resources with "Hres0") as (wastk) "[Hres0 $]". *)
-  (*       iDestruct (opening_closing_resources with "Hres1") as (wastk1) "[Hres1 $]". *)
-  (*       iDestruct (opening_closing_resources with "Hres2") as (wastk2) "[Hres2 $]". *)
-  (*       iDestruct (opening_closing_resources with "Hres3") as (wastk3) "[Hres3 $]". *)
-  (*       iFrame. *)
-  (*   } *)
-
-  (*   (* --- Load cgp csp --- *) *)
-  (*   iInstr "Hcode". *)
-  (*   { split ; [ solve_pure | rewrite le_addr_withinBounds ; solve_addr+Ha_stk4 Hb_a4 He_a1 ]. } *)
-  (*   iEval (cbn) in "Hcgp". *)
-
-  (*   (* --- Lea csp (-1)%Z --- *) *)
-  (*   iInstr "Hcode". *)
-  (*   { by transitivity (Some (a_stk ^+ 2)%a); solve_addr+Ha_stk4. } *)
-
-  (*   (* Load ca2 csp *) *)
-  (*   iInstr "Hcode". *)
-  (*   { split ; [ solve_pure | rewrite le_addr_withinBounds ; solve_addr+Ha_stk4 Hb_a4 He_a1 ]. } *)
-  (*   iEval (cbn) in "Hca2". *)
-  (*   (* Lea csp (-1)%Z *) *)
-  (*   iInstr "Hcode". *)
-  (*   { by transitivity (Some (a_stk ^+ 1)%a); solve_addr+Ha_stk4. } *)
-  (*   (* Load cs1 csp *) *)
-  (*   iInstr "Hcode". *)
-  (*   { split ; [ solve_pure | rewrite le_addr_withinBounds ; solve_addr+Ha_stk4 Hb_a4 He_a1 ]. } *)
-  (*   iEval (cbn) in "Hcs1". *)
-  (*   (* Lea csp (-1)%Z *) *)
-  (*   iInstr "Hcode". *)
-  (*   { by transitivity (Some a_stk); solve_addr. } *)
-  (*   (* Load cs0 csp *) *)
-  (*   iInstr "Hcode". *)
-  (*   { split ; [ solve_pure | rewrite le_addr_withinBounds ; solve_addr+Ha_stk4 Hb_a4 He_a1 ]. } *)
-  (*   iEval (cbn) in "Hcs0". *)
-  (*   (* GetE ct0 csp *) *)
-  (*   iInstr "Hcode". *)
-  (*   (* GetA ct1 csp *) *)
-  (*   iInstr "Hcode". *)
-
-  (*   unfocus_block "Hcode" "Hcont" as "Hcode"; subst hcont. *)
-
-  (*   { i} *)
-
-  (*   iAssert ( *)
-  (*       ∃ wastk wastk1 wastk2 wastk3, *)
-  (*       let la := (if is_untrusted_caller then finz.seq_between a_stk (a_stk ^+ 4)%a else []) in *)
-  (*       let lv := (if is_untrusted_caller then [wastk;wastk1;wastk2;wastk3] else []) in *)
-  (*         a_stk ↦ₐ wastk *)
-  (*         ∗ (a_stk ^+ 1)%a ↦ₐ wastk1 *)
-  (*         ∗ (a_stk ^+ 2)%a ↦ₐ wastk2 *)
-  (*         ∗ (a_stk ^+ 3)%a ↦ₐ wastk3 *)
-  (*         ∗ ▷ ([∗ list] a ; v ∈ la ; lv, ▷ closing_resources interp W C a v) *)
-  (*         ∗ ⌜if is_untrusted_caller then True else (wastk = wcs2 ∧ wastk1 = wcs3 ∧ wastk2 = wret ∧ wastk3 = wcgp0)⌝ *)
-  (*         ∗ open_region_many W C la *)
-  (*         ∗ sts_full_world W C *)
-  (*     )%I *)
-  (*     with "[Hcframe_interp Hr Hsts]" as "Hcframe_interp" *)
-  (*   ; [|iDestruct "Hcframe_interp" as *)
-  (*       (wastk wastk1 wastk2 wastk3) "(Ha_stk & Ha_stk1 & Ha_stk2 & Ha_stk3 & Hclose_res & %Hwastks & Hr & Hsts)" *)
-  (*     ]. *)
-
-
-  (*   iInstr "Hcode"; try solve_pure. *)
-
-
-  (*   [WriteSR mtdc ctp; Lea csp (-1)%Z; Load cgp csp; *)
-  (*    Lea csp (-1)%Z; Load ca2 csp; Lea csp (-1)%Z; Load cs1 csp; Lea csp (-1)%Z; Load cs0 csp; *)
-  (*    GetE ct0 csp; GetA ct1 csp] ++ *)
-  (* clear_stack_instrs ct0 ct1 ++ *)
-  (* encodeInstrsW [Mov cra ca2] ++ clear_registers_post_call_instrs ++ encodeInstrsW [JmpCap cra] *)
-
 
 
 
